Smt/Reconstruction/Rules.lean
@@ -11,74 +11,80 @@ namespace Rules
 
 syntax "absurdHyp" ident "(" ident,+ ")" : tactic
 macro_rules
-  | `(tactic| absurdHyp $h:ident ($n:ident)) => `(tactic| rewrite [($n)] at ($h); have z: False := ($h); cases z)
-  | `(tactic| absurdHyp $h:ident ($n:ident, $m:ident)) => `(tactic| rewrite [($n), ($m)] at ($h); have z: False := ($h); simp at z)
+  | `(tactic| absurdHyp $h:ident ($n:ident)) =>
+      `(tactic| rewrite [($n)] at ($h); have z: False := ($h); cases z)
+  | `(tactic| absurdHyp $h:ident ($n:ident, $m:ident)) =>
+      `(tactic| rewrite [($n), ($m)] at ($h); simp at ($h); exact False.elim (($h) True.intro))
 
 open Classical
 
+/- theorem notImplies1' : ∀ {t₁ t₂ : term}, -/
+/-   followsFrom (not $ implies t₁ t₂) t₁ := -/
+/-     by intros t₁ t₂ Γ Δ h -/
+/-        simp at h -/
+/-        split at h -/
+/-        case h_1 x k h' => -/
+/-          split at h' -/
+/-          case h_1 x' k' h'' => -/
+/-            split at h'' -/
+/-            case h_1 f k₁ k₂ h₁ h₂ => -/
+/-              have kk' : (fun Γ Δ => ¬ k' Γ Δ) = k := -/
+/-                by injection h' with _ z; exact z -/
+/-              have k'k₁k₂ : (λ Γ Δ => ((k₁ Γ Δ) → (k₂ Γ Δ))) = k' := -/
+/-                by injection h'' with _ z; exact z -/
+/-              rewrite [← k'k₁k₂] at kk' -/
+/-              simp -/
+/-              rewrite [h₁] -/
+/-              show Coe.coe (k₁ Γ Δ) -/
+/-              apply byContradiction -/
+/-              intro notk₁ -/
+/-              rewrite [← kk'] at h -/
+/-              exact h (λ k₁ => False.elim (notk₁ k₁)) -/
+/-            case h_2 x'' f h3 => -/
+/-              have k'T : (λ _ _ => True) = k' := -/
+/-                by injection h'' with _ z; exact z -/
+/-              rewrite [← k'T] at h' -/
+/-              have kF : (λ Γ Δ => ¬ (λ _ _ => True) Γ Δ) = k := -/
+/-                by injection h' with _ z; exact z -/
+/-              rewrite [← kF] at h -/
+/-              exact False.elim (h True.intro) -/
+/-          case h_2 k' h'' => admit -/
+/-        case h_2 x k => admit -/
+
 theorem notImplies1 : ∀ {t₁ t₂ : term},
   followsFrom (not $ implies t₁ t₂) t₁ :=
-  by intros t₁ t₂ Γ Δ h
-     simp at h
-     split at h
-     case h_1 _ k h' =>
-       split at h'
-       case h_1 _ k' h'' =>
-         split at h''
-         case h_1 _ k₁ k₂ rt₁ rt₂ =>
-           simp
-           rewrite [rt₁]
-           have ek : (fun Γ Δ => ¬ k' Γ Δ) = k :=
-             by injection h' with h'; injection h' with _ h'; exact h';
-           have fe : (fun Γ Δ => k₁ Γ Δ → k₂ Γ Δ) = k' :=
-             by injection h'' with h''; injection h'' with _ h''; exact h''
-           rewrite [← ek, ← fe] at h
+    by intros t₁ t₂ Γ Δ h
+       simp at *
+       match r₁: interpTerm t₁, r₂: interpTerm t₂ with
+       | ⟨ atom 1, k₁ ⟩, ⟨ atom 1, k₂ ⟩ =>
+         rewrite [r₁, r₂] at h
+         simp at h
+         have h' : ¬ (k₁ Γ Δ → k₂ Γ Δ) := h
+         simp
+         apply byContradiction
+         intro notk₁
+         exact False.elim (h' (λ k₁ => False.elim (notk₁ k₁)))
+       | ⟨ atom 0, _ ⟩, _  => simp
+       | ⟨ atom 1, k₁ ⟩, ⟨ atom 0, _ ⟩  => absurdHyp h (r₁, r₂)
+       | ⟨ atom 1, k₁ ⟩, ⟨ atom (succ (succ _)), _ ⟩ => absurdHyp h (r₁, r₂)
+       | ⟨ atom 1, k₁ ⟩, ⟨ sort.undef, _ ⟩           => absurdHyp h (r₁, r₂)
+       | ⟨ atom 1, k₁ ⟩, ⟨ sort.array _ _, _ ⟩       => absurdHyp h (r₁, r₂)
+       | ⟨ atom 1, k₁ ⟩, ⟨ sort.bv _, _ ⟩            => absurdHyp h (r₁, r₂)
+       | ⟨ atom 1, k₁ ⟩, ⟨ sort.arrow _ _, _ ⟩       => absurdHyp h (r₁, r₂)
+       | ⟨ atom 1, k₁ ⟩, ⟨ sort.dep, _ ⟩             => absurdHyp h (r₁, r₂)
+       | ⟨ atom (succ (succ _)), _ ⟩, _ => simp
+       | ⟨ sort.undef, _ ⟩, _           => simp
+       | ⟨ sort.array _ _, _ ⟩, _       => simp
+       | ⟨ sort.bv _, _ ⟩, _            => simp
+       | ⟨ sort.arrow _ _, _ ⟩, _       => simp
+       | ⟨ sort.dep, _ ⟩, _             => simp
 
-           apply byContradiction
-
-           exact (λ hf => h (λ k₁w => False.elim (hf k₁w)))
-         case h_2 => simp at h''
-       case h_2 => simp at h'
-     case h_2 => exact (False.elim h)
-
-/-      simp at * -/
-/-      split at h -/
-/-      case h_1 _ k h' => -/
-/-        split at h' -/
-/-        case h_1 _ k' h'' => -/
-/-          split at h'' -/
-/-          case h_1 _ k₁ k₂ rt₁ rt₂ => -/
-/-            split -/
-/-            case h_1 z q₁ i₂ k₂ h₂ aaaaaaa aaa aa => -/
-/-              rewrite [h₂] -/
-/-              have ek : (fun Γ Δ => ¬ k' Γ Δ) = k := -/
-/-                by injection h' with h'; injection h' with _ h'; exact h'; -/
-/-              have fe : (fun Γ Δ => k₁ Γ Δ → k₂ Γ Δ) = k' := -/
-/-                by injection h'' with h''; injection h'' with _ h''; exact h'' -/
-/-              rewrite [← ek, ← fe] at h -/
-             
-/-            case h_2 _ q₁ q₂ q₃ => admit -/
-           /- simp -/
-
-           /- rewrite [rt₂] -/
-           /- have ek : (fun Γ Δ => ¬ k' Γ Δ) = k := -/
-           /-   by injection h' with h'; injection h' with _ h'; exact h'; -/
-           /- have fe : (fun Γ Δ => k₁ Γ Δ → k₂ Γ Δ) = k' := -/
-           /-   by injection h'' with h''; injection h'' with _ h''; exact h'' -/
-           /- rewrite [← ek, ← fe] at h -/
-
-           /- apply byContradiction -/
-
-           /- exact (λ hf => h (λ k₁w => False.elim (hf k₁w))) -/
-         /- case h_2 => simp at h'' -/
-       /- case h_2 => simp at h' -/
-     /- case h_2 => exact (False.elim h) -/
 theorem notImplies2 : ∀ {t₁ t₂ : term},
   followsFrom (not $ implies t₁ t₂) (not t₂) :=
     by intros t₁ t₂ Γ Δ h
        simp at h
        match r₁: interpTerm t₁, r₂: interpTerm t₂ with
-       | some ⟨ atom 1, k₁ ⟩, some ⟨ atom 1, k₂ ⟩ =>
+       | ⟨ atom 1, k₁ ⟩, ⟨ atom 1, k₂ ⟩ =>
            simp
            rewrite [r₂]
            show ¬ k₂ Γ Δ
@@ -87,29 +93,35 @@ theorem notImplies2 : ∀ {t₁ t₂ : term},
            match em (k₂ Γ Δ) with
            | Or.inl r  => exact False.elim (h₂ (λ _ => r))
            | Or.inr r  => exact r
-       | some ⟨ atom 0, _ ⟩, _  => rewrite [r₁] at h; simp at h
-       | some ⟨ atom 1, k₁ ⟩, some ⟨ atom 0, _ ⟩  => absurdHyp h (r₁, r₂)
-       | some ⟨ atom 1, k₁ ⟩, some ⟨ atom (succ (succ _)), _ ⟩ => absurdHyp h (r₁, r₂)
-       | some ⟨ atom 1, k₁ ⟩, some ⟨ sort.undef, _ ⟩           => absurdHyp h (r₁, r₂)
-       | some ⟨ atom 1, k₁ ⟩, some ⟨ sort.array _ _, _ ⟩       => absurdHyp h (r₁, r₂)
-       | some ⟨ atom 1, k₁ ⟩, some ⟨ sort.bv _, _ ⟩            => absurdHyp h (r₁, r₂)
-       | some ⟨ atom 1, k₁ ⟩, some ⟨ sort.arrow _ _, _ ⟩       => absurdHyp h (r₁, r₂)
-       | some ⟨ atom 1, k₁ ⟩, some ⟨ sort.dep, _ ⟩             => absurdHyp h (r₁, r₂)
-       | some ⟨ atom 1, k₁ ⟩, none                             => absurdHyp h (r₁, r₂)
-       | some ⟨ atom (succ (succ _)), _ ⟩, _ => absurdHyp h (r₁) 
-       | some ⟨ sort.undef, _ ⟩, _           => absurdHyp h (r₁) 
-       | some ⟨ sort.array _ _, _ ⟩, _       => absurdHyp h (r₁) 
-       | some ⟨ sort.bv _, _ ⟩, _            => absurdHyp h (r₁) 
-       | some ⟨ sort.arrow _ _, _ ⟩, _       => absurdHyp h (r₁) 
-       | some ⟨ sort.dep, _ ⟩, _             => absurdHyp h (r₁)
-       | none, _                             => absurdHyp h (r₁)
+       | _, ⟨ atom 0, _ ⟩               => simp; rewrite [r₂]; exact True.intro
+       | _, ⟨ atom (succ (succ _)), _ ⟩ => simp; rewrite [r₂]; exact True.intro
+       | _, ⟨ sort.undef, _ ⟩           => simp; rewrite [r₂]; exact True.intro
+       | _, ⟨ sort.array _ _, _ ⟩       => simp; rewrite [r₂]; exact True.intro
+       | _, ⟨ sort.dep, _ ⟩             => simp; rewrite [r₂]; exact True.intro
+       | _, ⟨ sort.bv _, _ ⟩            => simp; rewrite [r₂]; exact True.intro
+       | _, ⟨ sort.arrow _ _, _ ⟩       => simp; rewrite [r₂]; exact True.intro
+       | ⟨ atom 0, _ ⟩, ⟨ atom 1, k₂ ⟩               => absurdHyp h (r₁, r₂)
+       | ⟨ atom (succ (succ _)), _ ⟩, ⟨ atom 1, k₂ ⟩ => absurdHyp h (r₁, r₂)
+       | ⟨ sort.undef, _ ⟩, ⟨ atom 1, k₂ ⟩           => absurdHyp h (r₁, r₂)
+       | ⟨ sort.array _ _, _ ⟩, ⟨ atom 1, k₂ ⟩       => absurdHyp h (r₁, r₂)
+       | ⟨ sort.dep, _ ⟩, ⟨ atom 1, k₂ ⟩             => absurdHyp h (r₁, r₂)
+       | ⟨ sort.bv _, _ ⟩, ⟨ atom 1, k₂ ⟩            => absurdHyp h (r₁, r₂)
+       | ⟨ sort.arrow _ _, _ ⟩, ⟨ atom 1, k₂ ⟩       => absurdHyp h (r₁, r₂)
 
+
+/- theorem orIntro : ∀ {t₁ t₂ : term}, -/
+/-   followsFrom t₁ (or t₂ t₁) -/
+/-   | t₁, t₂, Γ, Δ, h => -/
+/-     by simp at h -/
+/-        simp -/
+
+-- t1 mal formado e t2 falso? -> absurdHyp
 theorem impliesElim : ∀ {t₁ t₂ : term},
   followsFrom (implies t₁ t₂) (or (not t₁) t₂)
   | t₁, t₂, Γ, Δ, h =>
     by simp at h
        match r₁: interpTerm t₁, r₂: interpTerm t₂ with
-       | some ⟨ atom 1, k₁ ⟩, some ⟨ atom 1, k₂ ⟩ =>
+       | ⟨ atom 1, k₁ ⟩, ⟨ atom 1, k₂ ⟩ =>
            simp
            rewrite [r₁, r₂]
            rewrite [r₁, r₂] at h
@@ -121,137 +133,138 @@ theorem impliesElim : ∀ {t₁ t₂ : term},
                                         exact (False.elim (nk₂W k₂W))
            | Or.inr _, Or.inl k₂W => exact Or.inr k₂W
            | Or.inr nk₁W, Or.inr _ => exact Or.inl nk₁W
-       | some ⟨ atom 0, _ ⟩, _  => absurdHyp h (r₁)
-       | some ⟨ atom 1, k₁ ⟩, some ⟨ atom 0, _ ⟩  => absurdHyp h (r₁, r₂)
-       | some ⟨ atom 1, k₁ ⟩, some ⟨ atom (succ (succ _)), _ ⟩ => absurdHyp h (r₁, r₂)
-       | some ⟨ atom 1, k₁ ⟩, some ⟨ sort.undef, _ ⟩           => absurdHyp h (r₁, r₂)
-       | some ⟨ atom 1, k₁ ⟩, some ⟨ sort.array _ _, _ ⟩       => absurdHyp h (r₁, r₂)
-       | some ⟨ atom 1, k₁ ⟩, some ⟨ sort.bv _, _ ⟩            => absurdHyp h (r₁, r₂)
-       | some ⟨ atom 1, k₁ ⟩, some ⟨ sort.arrow _ _, _ ⟩       => absurdHyp h (r₁, r₂)
-       | some ⟨ atom 1, k₁ ⟩, some ⟨ sort.dep, _ ⟩             => absurdHyp h (r₁, r₂)
-       | some ⟨ atom 1, k₁ ⟩, none                             => absurdHyp h (r₁, r₂)
-       | some ⟨ atom (succ (succ _)), _ ⟩, _ => absurdHyp h (r₁) 
-       | some ⟨ sort.undef, _ ⟩, _           => absurdHyp h (r₁) 
-       | some ⟨ sort.array _ _, _ ⟩, _       => absurdHyp h (r₁)
-       | some ⟨ sort.bv _, _ ⟩, _            => absurdHyp h (r₁)
-       | some ⟨ sort.arrow _ _, _ ⟩, _       => absurdHyp h (r₁)
-       | some ⟨ sort.dep, _ ⟩, _             => absurdHyp h (r₁)
-       | none, _                             => absurdHyp h (r₁)
+       | _, _ => admit
+/-        | some ⟨ atom 0, _ ⟩, _  => absurdHyp h (r₁) -/
+/-        | some ⟨ atom 1, k₁ ⟩, some ⟨ atom 0, _ ⟩  => absurdHyp h (r₁, r₂) -/
+/-        | some ⟨ atom 1, k₁ ⟩, some ⟨ atom (succ (succ _)), _ ⟩ => absurdHyp h (r₁, r₂) -/
+/-        | some ⟨ atom 1, k₁ ⟩, some ⟨ sort.undef, _ ⟩           => absurdHyp h (r₁, r₂) -/
+/-        | some ⟨ atom 1, k₁ ⟩, some ⟨ sort.array _ _, _ ⟩       => absurdHyp h (r₁, r₂) -/
+/-        | some ⟨ atom 1, k₁ ⟩, some ⟨ sort.bv _, _ ⟩            => absurdHyp h (r₁, r₂) -/
+/-        | some ⟨ atom 1, k₁ ⟩, some ⟨ sort.arrow _ _, _ ⟩       => absurdHyp h (r₁, r₂) -/
+/-        | some ⟨ atom 1, k₁ ⟩, some ⟨ sort.dep, _ ⟩             => absurdHyp h (r₁, r₂) -/
+/-        | some ⟨ atom 1, k₁ ⟩, none                             => absurdHyp h (r₁, r₂) -/
+/-        | some ⟨ atom (succ (succ _)), _ ⟩, _ => absurdHyp h (r₁) -/ 
+/-        | some ⟨ sort.undef, _ ⟩, _           => absurdHyp h (r₁) -/ 
+/-        | some ⟨ sort.array _ _, _ ⟩, _       => absurdHyp h (r₁) -/
+/-        | some ⟨ sort.bv _, _ ⟩, _            => absurdHyp h (r₁) -/
+/-        | some ⟨ sort.arrow _ _, _ ⟩, _       => absurdHyp h (r₁) -/
+/-        | some ⟨ sort.dep, _ ⟩, _             => absurdHyp h (r₁) -/
+/-        | none, _                             => absurdHyp h (r₁) -/
 
-theorem contradiction: ∀ {t: term},
-  followsFrom (and (not t) t) bot
-  | t, Γ, Δ, h => by
-    simp at h
-    match r: interpTerm t with
-    | some ⟨ atom 1, k ⟩ =>
-        rewrite [r] at h;
-        simp at h
-        have ⟨nkW, kW⟩ : ¬ (k Γ Δ) ∧ k Γ Δ := h
-        exact False.elim (nkW kW)
-    | some ⟨ atom 0, _ ⟩               => absurdHyp h (r)
-    | some ⟨ atom (succ (succ _)), _ ⟩ => absurdHyp h (r)
-    | some ⟨ sort.undef, _ ⟩           => absurdHyp h (r)
-    | some ⟨ sort.array _ _, _ ⟩       => absurdHyp h (r)
-    | some ⟨ sort.bv _, _ ⟩            => absurdHyp h (r)
-    | some ⟨ sort.arrow _ _, _ ⟩       => absurdHyp h (r)
-    | some ⟨ sort.dep, _ ⟩             => absurdHyp h (r)
-    | none                             => absurdHyp h (r)
+/- theorem contradiction: ∀ {t: term}, -/
+/-   followsFrom (and (not t) t) bot -/
+/-   | t, Γ, Δ, h => by -/
+/-     simp at h -/
+/-     match r: interpTerm t with -/
+/-     | some ⟨ atom 1, k ⟩ => -/
+/-         rewrite [r] at h; -/
+/-         simp at h -/
+/-         have ⟨nkW, kW⟩ : ¬ (k Γ Δ) ∧ k Γ Δ := h -/
+/-         exact False.elim (nkW kW) -/
+/-     | some ⟨ atom 0, _ ⟩               => absurdHyp h (r) -/
+/-     | some ⟨ atom (succ (succ _)), _ ⟩ => absurdHyp h (r) -/
+/-     | some ⟨ sort.undef, _ ⟩           => absurdHyp h (r) -/
+/-     | some ⟨ sort.array _ _, _ ⟩       => absurdHyp h (r) -/
+/-     | some ⟨ sort.bv _, _ ⟩            => absurdHyp h (r) -/
+/-     | some ⟨ sort.arrow _ _, _ ⟩       => absurdHyp h (r) -/
+/-     | some ⟨ sort.dep, _ ⟩             => absurdHyp h (r) -/
+/-     | none                             => absurdHyp h (r) -/
        
-theorem R1 : ∀ {t₁ t₂ : term},
-  followsFrom (and (or (not t₁) t₂) t₁) t₂
-  | t₁, t₂, Γ, Δ, h => by
-    simp at h
-    match r₁: interpTerm t₁, r₂: interpTerm t₂ with
-    | some ⟨ atom 1, k₁ ⟩, some ⟨ atom 1, k₂ ⟩ =>
-        simp at *
-        rewrite [r₁, r₂] at h
-        rewrite [r₂]
-        have ⟨ H, k₁W ⟩: ((¬ (k₁ Γ Δ)) ∨ (k₂ Γ Δ)) ∧ (k₁ Γ Δ) := h
-        match em (k₂ Γ Δ) with
-        | Or.inl k₂W  => exact k₂W
-        | Or.inr nk₂W => match em (k₁ Γ Δ) with
-                         | Or.inl k₁W  => match H with
-                                          | Or.inl nk₁W => exact (False.elim (nk₁W k₁W))
-                                          | Or.inr k₂W  => exact k₂W
-                         | Or.inr nk₁W => exact (False.elim (nk₁W k₁W))
-    | some ⟨ atom 1, _ ⟩, some ⟨ atom 0, _ ⟩               => absurdHyp h (r₁, r₂)
-    | some ⟨ atom 1, _ ⟩, some ⟨ atom (succ (succ _)), _ ⟩ => absurdHyp h (r₁, r₂)
-    | some ⟨ atom 1, _ ⟩, some ⟨ sort.undef, _ ⟩           => absurdHyp h (r₁, r₂)
-    | some ⟨ atom 1, _ ⟩, some ⟨ sort.array _ _, _ ⟩       => absurdHyp h (r₁, r₂)
-    | some ⟨ atom 1, _ ⟩, some ⟨ sort.bv _, _ ⟩            => absurdHyp h (r₁, r₂)
-    | some ⟨ atom 1, _ ⟩, some ⟨ sort.arrow _ _, _ ⟩       => absurdHyp h (r₁, r₂)
-    | some ⟨ atom 1, _ ⟩, some ⟨ sort.dep, _ ⟩             => absurdHyp h (r₁, r₂)
-    | some ⟨ atom 1, _ ⟩, none                             => absurdHyp h (r₁, r₂)
-    | some ⟨ atom 0, _ ⟩, _               => absurdHyp h (r₁) 
-    | some ⟨ atom (succ (succ _)), _ ⟩, _ => absurdHyp h (r₁)
-    | some ⟨ sort.undef, _ ⟩, _           => absurdHyp h (r₁)
-    | some ⟨ sort.array _ _, _ ⟩, _       => absurdHyp h (r₁)
-    | some ⟨ sort.bv _, _ ⟩, _            => absurdHyp h (r₁)
-    | some ⟨ sort.arrow _ _, _ ⟩, _       => absurdHyp h (r₁)
-    | some ⟨ sort.dep, _ ⟩, _             => absurdHyp h (r₁)
-    | none, _                             => absurdHyp h (r₁)
+/- theorem R1 : ∀ {t₁ t₂ : term}, -/
+/-   followsFrom (and (or (not t₁) t₂) t₁) t₂ -/
+/-   | t₁, t₂, Γ, Δ, h => by -/
+/-     simp at h -/
+/-     match r₁: interpTerm t₁, r₂: interpTerm t₂ with -/
+/-     | some ⟨ atom 1, k₁ ⟩, some ⟨ atom 1, k₂ ⟩ => -/
+/-         simp at * -/
+/-         rewrite [r₁, r₂] at h -/
+/-         rewrite [r₂] -/
+/-         have ⟨ H, k₁W ⟩: ((¬ (k₁ Γ Δ)) ∨ (k₂ Γ Δ)) ∧ (k₁ Γ Δ) := h -/
+/-         match em (k₂ Γ Δ) with -/
+/-         | Or.inl k₂W  => exact k₂W -/
+/-         | Or.inr nk₂W => match em (k₁ Γ Δ) with -/
+/-                          | Or.inl k₁W  => match H with -/
+/-                                           | Or.inl nk₁W => exact (False.elim (nk₁W k₁W)) -/
+/-                                           | Or.inr k₂W  => exact k₂W -/
+/-                          | Or.inr nk₁W => exact (False.elim (nk₁W k₁W)) -/
+/-     | some ⟨ atom 1, _ ⟩, some ⟨ atom 0, _ ⟩               => absurdHyp h (r₁, r₂) -/
+/-     | some ⟨ atom 1, _ ⟩, some ⟨ atom (succ (succ _)), _ ⟩ => absurdHyp h (r₁, r₂) -/
+/-     | some ⟨ atom 1, _ ⟩, some ⟨ sort.undef, _ ⟩           => absurdHyp h (r₁, r₂) -/
+/-     | some ⟨ atom 1, _ ⟩, some ⟨ sort.array _ _, _ ⟩       => absurdHyp h (r₁, r₂) -/
+/-     | some ⟨ atom 1, _ ⟩, some ⟨ sort.bv _, _ ⟩            => absurdHyp h (r₁, r₂) -/
+/-     | some ⟨ atom 1, _ ⟩, some ⟨ sort.arrow _ _, _ ⟩       => absurdHyp h (r₁, r₂) -/
+/-     | some ⟨ atom 1, _ ⟩, some ⟨ sort.dep, _ ⟩             => absurdHyp h (r₁, r₂) -/
+/-     | some ⟨ atom 1, _ ⟩, none                             => absurdHyp h (r₁, r₂) -/
+/-     | some ⟨ atom 0, _ ⟩, _               => absurdHyp h (r₁) -/ 
+/-     | some ⟨ atom (succ (succ _)), _ ⟩, _ => absurdHyp h (r₁) -/
+/-     | some ⟨ sort.undef, _ ⟩, _           => absurdHyp h (r₁) -/
+/-     | some ⟨ sort.array _ _, _ ⟩, _       => absurdHyp h (r₁) -/
+/-     | some ⟨ sort.bv _, _ ⟩, _            => absurdHyp h (r₁) -/
+/-     | some ⟨ sort.arrow _ _, _ ⟩, _       => absurdHyp h (r₁) -/
+/-     | some ⟨ sort.dep, _ ⟩, _             => absurdHyp h (r₁) -/
+/-     | none, _                             => absurdHyp h (r₁) -/
 
-theorem conjunction: ∀ {t₁ t₂: term} {Γ: Environment} {Δ : SEnvironment},
-  validWith Γ Δ t₁ → validWith Γ Δ t₂ → validWith Γ Δ (and t₁ t₂)
-  | t₁, t₂, Γ, Δ, h₁, h₂ => by
-    simp at *
-    match r₁: interpTerm t₁, r₂: interpTerm t₂ with
-    | some ⟨ atom 1, k₁ ⟩, some ⟨ atom 1, k₂ ⟩ =>
-        show (k₁ Γ Δ) ∧ (k₂ Γ Δ)
-        simp
-        rewrite [r₁] at h₁
-        rewrite [r₂] at h₂
-        have k₁W: (k₁ Γ Δ) := h₁
-        have k₂W: (k₂ Γ Δ) := h₂
-        exact And.intro k₁W k₂W
-    | some ⟨ atom 1, _ ⟩, some ⟨ atom 0, _ ⟩               => absurdHyp h₂ (r₂)
-    | some ⟨ atom 1, _ ⟩, some ⟨ atom (succ (succ _)), _ ⟩ => absurdHyp h₂ (r₂)
-    | some ⟨ atom 1, _ ⟩, some ⟨ sort.undef, _ ⟩           => absurdHyp h₂ (r₂)
-    | some ⟨ atom 1, _ ⟩, some ⟨ sort.array _ _, _ ⟩       => absurdHyp h₂ (r₂)
-    | some ⟨ atom 1, _ ⟩, some ⟨ sort.bv _, _ ⟩            => absurdHyp h₂ (r₂)
-    | some ⟨ atom 1, _ ⟩, some ⟨ sort.arrow _ _, _ ⟩       => absurdHyp h₂ (r₂)
-    | some ⟨ atom 1, _ ⟩, some ⟨ sort.dep, _ ⟩             => absurdHyp h₂ (r₂)
-    | some ⟨ atom 1, _ ⟩, none                             => absurdHyp h₂ (r₂)
-    | some ⟨ atom 0, _ ⟩, _                                => absurdHyp h₁ (r₁)
-    | some ⟨ atom (succ (succ _)), _ ⟩ , _ => absurdHyp h₁ (r₁)
-    | some ⟨ sort.undef, _ ⟩, _            => absurdHyp h₁ (r₁)
-    | some ⟨ sort.array _ _, _ ⟩, _        => absurdHyp h₁ (r₁)
-    | some ⟨ sort.bv _, _ ⟩, _             => absurdHyp h₁ (r₁)
-    | some ⟨ sort.arrow _ _, _ ⟩, _        => absurdHyp h₁ (r₁)
-    | some ⟨ sort.dep, _ ⟩, _              => absurdHyp h₁ (r₁)
-    | none, _                              => absurdHyp h₁ (r₁)
+/- theorem conjunction: ∀ {t₁ t₂: term} {Γ: Environment} {Δ : SEnvironment}, -/
+/-   validWith Γ Δ t₁ → validWith Γ Δ t₂ → validWith Γ Δ (and t₁ t₂) -/
+/-   | t₁, t₂, Γ, Δ, h₁, h₂ => by -/
+/-     simp at * -/
+/-     match r₁: interpTerm t₁, r₂: interpTerm t₂ with -/
+/-     | some ⟨ atom 1, k₁ ⟩, some ⟨ atom 1, k₂ ⟩ => -/
+/-         show (k₁ Γ Δ) ∧ (k₂ Γ Δ) -/
+/-         simp -/
+/-         rewrite [r₁] at h₁ -/
+/-         rewrite [r₂] at h₂ -/
+/-         have k₁W: (k₁ Γ Δ) := h₁ -/
+/-         have k₂W: (k₂ Γ Δ) := h₂ -/
+/-         exact And.intro k₁W k₂W -/
+/-     | some ⟨ atom 1, _ ⟩, some ⟨ atom 0, _ ⟩               => absurdHyp h₂ (r₂) -/
+/-     | some ⟨ atom 1, _ ⟩, some ⟨ atom (succ (succ _)), _ ⟩ => absurdHyp h₂ (r₂) -/
+/-     | some ⟨ atom 1, _ ⟩, some ⟨ sort.undef, _ ⟩           => absurdHyp h₂ (r₂) -/
+/-     | some ⟨ atom 1, _ ⟩, some ⟨ sort.array _ _, _ ⟩       => absurdHyp h₂ (r₂) -/
+/-     | some ⟨ atom 1, _ ⟩, some ⟨ sort.bv _, _ ⟩            => absurdHyp h₂ (r₂) -/
+/-     | some ⟨ atom 1, _ ⟩, some ⟨ sort.arrow _ _, _ ⟩       => absurdHyp h₂ (r₂) -/
+/-     | some ⟨ atom 1, _ ⟩, some ⟨ sort.dep, _ ⟩             => absurdHyp h₂ (r₂) -/
+/-     | some ⟨ atom 1, _ ⟩, none                             => absurdHyp h₂ (r₂) -/
+/-     | some ⟨ atom 0, _ ⟩, _                                => absurdHyp h₁ (r₁) -/
+/-     | some ⟨ atom (succ (succ _)), _ ⟩ , _ => absurdHyp h₁ (r₁) -/
+/-     | some ⟨ sort.undef, _ ⟩, _            => absurdHyp h₁ (r₁) -/
+/-     | some ⟨ sort.array _ _, _ ⟩, _        => absurdHyp h₁ (r₁) -/
+/-     | some ⟨ sort.bv _, _ ⟩, _             => absurdHyp h₁ (r₁) -/
+/-     | some ⟨ sort.arrow _ _, _ ⟩, _        => absurdHyp h₁ (r₁) -/
+/-     | some ⟨ sort.dep, _ ⟩, _              => absurdHyp h₁ (r₁) -/
+/-     | none, _                              => absurdHyp h₁ (r₁) -/
 
-theorem followsBot: ∀ {t: term},
-  followsFrom t bot → ∀ {Γ : Environment} {Δ : SEnvironment}, ¬ validWith Γ Δ t
-  | t, h, Γ, Δ => by
-    intro validT
-    have validBot := @h Γ Δ validT
-    simp at validBot
-    cases validBot
+/- theorem followsBot: ∀ {t: term}, -/
+/-   followsFrom t bot → ∀ {Γ : Environment} {Δ : SEnvironment}, ¬ validWith Γ Δ t -/
+/-   | t, h, Γ, Δ => by -/
+/-     intro validT -/
+/-     have validBot := @h Γ Δ validT -/
+/-     simp at validBot -/
+/-     cases validBot -/
 
-@[simp] def isBool : term → Bool
-  | t => match interpTerm t with
-         | some ⟨ atom 1, _ ⟩ => true
-         | _ => false
+/- @[simp] def isBool : term → Bool -/
+/-   | t => match interpTerm t with -/
+/-          | some ⟨ atom 1, _ ⟩ => true -/
+/-          | _ => false -/
 
-theorem interpNotTerm: ∀ {Γ: Environment} {Δ: SEnvironment} {t: term},
-  isBool t → ¬ validWith Γ Δ (not t) → validWith Γ Δ t
-  | Γ, Δ, t, bt, h => by
-    simp
-    match r: interpTerm t with
-    | some ⟨ atom 1, k ⟩ => match em (k Γ Δ) with
-                            | Or.inl kW  => exact kW
-                            | Or.inr nkW => simp at h
-                                            rewrite [r] at h
-                                            have nnkW : ¬ (¬ (k Γ Δ)) := h
-                                            exact (False.elim (nnkW nkW))
-    | some ⟨ atom 0, _ ⟩               => simp at bt; rewrite [r] at bt; cases bt
-    | some ⟨ atom (succ (succ _)), _ ⟩ => simp at bt; rewrite [r] at bt; cases bt
-    | some ⟨ sort.undef, _ ⟩           => simp at bt; rewrite [r] at bt; cases bt
-    | some ⟨ sort.array _ _, _ ⟩       => simp at bt; rewrite [r] at bt; cases bt
-    | some ⟨ sort.bv _, _ ⟩            => simp at bt; rewrite [r] at bt; cases bt
-    | some ⟨ sort.arrow _ _, _ ⟩       => simp at bt; rewrite [r] at bt; cases bt
-    | some ⟨ sort.dep, _ ⟩             => simp at bt; rewrite [r] at bt; cases bt
-    | none                             => simp at bt; rewrite [r] at bt; cases bt
+/- theorem interpNotTerm: ∀ {Γ: Environment} {Δ: SEnvironment} {t: term}, -/
+/-   isBool t → ¬ validWith Γ Δ (not t) → validWith Γ Δ t -/
+/-   | Γ, Δ, t, bt, h => by -/
+/-     simp -/
+/-     match r: interpTerm t with -/
+/-     | some ⟨ atom 1, k ⟩ => match em (k Γ Δ) with -/
+/-                             | Or.inl kW  => exact kW -/
+/-                             | Or.inr nkW => simp at h -/
+/-                                             rewrite [r] at h -/
+/-                                             have nnkW : ¬ (¬ (k Γ Δ)) := h -/
+/-                                             exact (False.elim (nnkW nkW)) -/
+/-     | some ⟨ atom 0, _ ⟩               => simp at bt; rewrite [r] at bt; cases bt -/
+/-     | some ⟨ atom (succ (succ _)), _ ⟩ => simp at bt; rewrite [r] at bt; cases bt -/
+/-     | some ⟨ sort.undef, _ ⟩           => simp at bt; rewrite [r] at bt; cases bt -/
+/-     | some ⟨ sort.array _ _, _ ⟩       => simp at bt; rewrite [r] at bt; cases bt -/
+/-     | some ⟨ sort.bv _, _ ⟩            => simp at bt; rewrite [r] at bt; cases bt -/
+/-     | some ⟨ sort.arrow _ _, _ ⟩       => simp at bt; rewrite [r] at bt; cases bt -/
+/-     | some ⟨ sort.dep, _ ⟩             => simp at bt; rewrite [r] at bt; cases bt -/
+/-     | none                             => simp at bt; rewrite [r] at bt; cases bt -/
 
 end Rules
