Smt/Reconstruction/Utils.lean
@@ -1,3 +1,0 @@
-@[simp] def isSome : Option α → Prop
-| none => False
-| some _ => True
